Need some lemmas for Patterns/ check shift problem for CaseV

2016/Ext_Structures.thy
@@ -143,156 +143,159 @@ text{*  For the typing rule of letbinder, we require to replace the type
 inductive has_type_L :: "lcontext \<Rightarrow> lterm \<Rightarrow> pcontext \<Rightarrow> ltype \<Rightarrow> bool" ("((_)/ \<turnstile> \<lparr>(_)|;|(_)\<rparr>/ |:| (_))" [150, 150, 150, 150] 150) where
   -- "Rules relating to the type of Booleans"
   has_type_LTrue:
-    "\<Gamma> \<turnstile> \<lparr>LTrue|;|fill \<delta>\<rparr> |:| Bool" |
+    "\<Gamma> \<turnstile> \<lparr>LTrue|;|fill \<sigma>\<rparr> |:| Bool" |
   has_type_LFalse:
-    "\<Gamma> \<turnstile> \<lparr>LFalse|;|fill \<delta>\<rparr> |:| Bool" |
+    "\<Gamma> \<turnstile> \<lparr>LFalse|;|fill \<sigma>\<rparr> |:| Bool" |
   has_type_LIf:
-    "\<Gamma> \<turnstile> \<lparr>t1|;|fill \<delta>\<rparr> |:| Bool \<Longrightarrow> \<Gamma> \<turnstile> \<lparr>t2|;|fill \<delta>\<rparr> |:| T' \<Longrightarrow> \<Gamma> \<turnstile> \<lparr>t3|;|fill \<delta>\<rparr> |:| T' \<Longrightarrow> \<Gamma> \<turnstile> \<lparr>LIf t1 t2 t3|;|fill \<delta>\<rparr> |:| T'" |
+    "\<Gamma> \<turnstile> \<lparr>t1|;|fill \<sigma>\<rparr> |:| Bool \<Longrightarrow> \<Gamma> \<turnstile> \<lparr>t2|;|fill \<sigma>\<rparr> |:| T' \<Longrightarrow> \<Gamma> \<turnstile> \<lparr>t3|;|fill \<sigma>\<rparr> |:| T' \<Longrightarrow> \<Gamma> \<turnstile> \<lparr>LIf t1 t2 t3|;|fill \<sigma>\<rparr> |:| T'" |
 
   -- \<open>Rules relating to the type of the constructs of the $\lambda$-calculus\<close>
   has_type_LVar:
-    "(x, T') |\<in>| \<Gamma> \<Longrightarrow> \<Gamma> \<turnstile> \<lparr>LVar x|;|fill \<delta>\<rparr> |:| (T')" |
+    "(x, T') |\<in>| \<Gamma> \<Longrightarrow> \<Gamma> \<turnstile> \<lparr>LVar x|;|fill \<sigma>\<rparr> |:| (T')" |
   has_type_LNat:
-    "\<Gamma> \<turnstile> \<lparr>LNat n|;| fill \<delta>\<rparr> |:| Nat"|
+    "\<Gamma> \<turnstile> \<lparr>LNat n|;| fill \<sigma>\<rparr> |:| Nat"|
   has_type_LPlus:
-    "\<Gamma> \<turnstile> \<lparr>t1|;| fill \<delta>\<rparr> |:| Nat \<Longrightarrow> \<Gamma> \<turnstile> \<lparr>t2|;| fill \<delta>\<rparr> |:| Nat \<Longrightarrow> \<Gamma> \<turnstile> \<lparr>LPlus t1 t2|;| fill \<delta>\<rparr> |:| Nat" |  
+    "\<Gamma> \<turnstile> \<lparr>t1|;| fill \<sigma>\<rparr> |:| Nat \<Longrightarrow> \<Gamma> \<turnstile> \<lparr>t2|;| fill \<sigma>\<rparr> |:| Nat \<Longrightarrow> \<Gamma> \<turnstile> \<lparr>LPlus t1 t2|;| fill \<sigma>\<rparr> |:| Nat" |  
   has_type_UMinus:
-    "\<Gamma> \<turnstile> \<lparr>t|;| fill \<delta>\<rparr> |:| Nat \<Longrightarrow> \<Gamma> \<turnstile> \<lparr>UMinus t|;| fill \<delta>\<rparr> |:| Nat" |
+    "\<Gamma> \<turnstile> \<lparr>t|;| fill \<sigma>\<rparr> |:| Nat \<Longrightarrow> \<Gamma> \<turnstile> \<lparr>UMinus t|;| fill \<sigma>\<rparr> |:| Nat" |
   has_type_IsZero:
-    "\<Gamma> \<turnstile> \<lparr>t|;| fill \<delta>\<rparr> |:| Nat \<Longrightarrow> \<Gamma> \<turnstile> \<lparr>IsZero t|;| fill \<delta>\<rparr> |:| Bool" |
+    "\<Gamma> \<turnstile> \<lparr>t|;| fill \<sigma>\<rparr> |:| Nat \<Longrightarrow> \<Gamma> \<turnstile> \<lparr>IsZero t|;| fill \<sigma>\<rparr> |:| Bool" |
   has_type_LAbs:
-    "(\<Gamma> |,| T1) \<turnstile> \<lparr>t2|;| fill \<delta>\<rparr> |:| T2 \<Longrightarrow> \<Gamma> \<turnstile> \<lparr>LAbs T1 t2|;|fill \<delta>\<rparr> |:| (T1 \<rightarrow> T2)" |
+    "(\<Gamma> |,| T1) \<turnstile> \<lparr>t2|;| fill \<sigma>\<rparr> |:| T2 \<Longrightarrow> \<Gamma> \<turnstile> \<lparr>LAbs T1 t2|;|fill \<sigma>\<rparr> |:| (T1 \<rightarrow> T2)" |
   has_type_LApp:
-    "\<Gamma> \<turnstile> \<lparr>t1|;|fill \<delta>\<rparr> |:| (T11 \<rightarrow> T12) \<Longrightarrow> \<Gamma> \<turnstile> \<lparr>t2|;|fill \<delta>\<rparr> |:| T11 \<Longrightarrow> \<Gamma> \<turnstile> \<lparr>LApp t1 t2|;|fill \<delta>\<rparr> |:| T12" |  
+    "\<Gamma> \<turnstile> \<lparr>t1|;|fill \<sigma>\<rparr> |:| (T11 \<rightarrow> T12) \<Longrightarrow> \<Gamma> \<turnstile> \<lparr>t2|;|fill \<sigma>\<rparr> |:| T11 \<Longrightarrow> \<Gamma> \<turnstile> \<lparr>LApp t1 t2|;|fill \<sigma>\<rparr> |:| T12" |  
   has_type_LUnit:
-    "\<Gamma> \<turnstile> \<lparr>unit|;|fill \<delta>\<rparr> |:| Unit " |  
+    "\<Gamma> \<turnstile> \<lparr>unit|;|fill \<sigma>\<rparr> |:| Unit " |  
   has_type_LSeq:
-    "\<Gamma> \<turnstile> \<lparr>t1|;|fill \<delta>\<rparr> |:| Unit \<Longrightarrow> \<Gamma> \<turnstile> \<lparr>t2|;|fill \<delta>\<rparr> |:| A \<Longrightarrow> \<Gamma> \<turnstile> \<lparr>Seq t1 t2|;|fill \<delta>\<rparr> |:| A" |
+    "\<Gamma> \<turnstile> \<lparr>t1|;|fill \<sigma>\<rparr> |:| Unit \<Longrightarrow> \<Gamma> \<turnstile> \<lparr>t2|;|fill \<sigma>\<rparr> |:| A \<Longrightarrow> \<Gamma> \<turnstile> \<lparr>Seq t1 t2|;|fill \<sigma>\<rparr> |:| A" |
   has_type_LAscribe:
-    "\<Gamma> \<turnstile> \<lparr>t1|;|fill \<delta>\<rparr> |:| A \<Longrightarrow> \<Gamma> \<turnstile> \<lparr>t1 as A|;|fill \<delta>\<rparr> |:| A" |
+    "\<Gamma> \<turnstile> \<lparr>t1|;|fill \<sigma>\<rparr> |:| A \<Longrightarrow> \<Gamma> \<turnstile> \<lparr>t1 as A|;|fill \<sigma>\<rparr> |:| A" |
   has_type_Let:
-    "\<Gamma> \<turnstile> \<lparr>t1|;|fill \<delta>\<rparr> |:| A \<Longrightarrow> (insert_nth x A \<Gamma>) \<turnstile> \<lparr> t2|;| fill \<delta>\<rparr> |:| B \<Longrightarrow> \<Gamma> \<turnstile> \<lparr>Let var x := t1 in t2|;|fill \<delta>\<rparr> |:| B" |
+    "\<Gamma> \<turnstile> \<lparr>t1|;|fill \<sigma>\<rparr> |:| A \<Longrightarrow> (insert_nth x A \<Gamma>) \<turnstile> \<lparr> t2|;| fill \<sigma>\<rparr> |:| B \<Longrightarrow> \<Gamma> \<turnstile> \<lparr>Let var x := t1 in t2|;|fill \<sigma>\<rparr> |:| B" |
   has_type_Pair:
-    "\<Gamma> \<turnstile> \<lparr>t1|;|fill \<delta>\<rparr> |:| A \<Longrightarrow> \<Gamma> \<turnstile> \<lparr>t2|;|fill \<delta>\<rparr> |:| B \<Longrightarrow> \<Gamma> \<turnstile> \<lparr>\<lbrace>t1,t2\<rbrace>|;|fill \<delta>\<rparr> |:| A |\<times>| B" |
+    "\<Gamma> \<turnstile> \<lparr>t1|;|fill \<sigma>\<rparr> |:| A \<Longrightarrow> \<Gamma> \<turnstile> \<lparr>t2|;|fill \<sigma>\<rparr> |:| B \<Longrightarrow> \<Gamma> \<turnstile> \<lparr>\<lbrace>t1,t2\<rbrace>|;|fill \<sigma>\<rparr> |:| A |\<times>| B" |
   has_type_Proj1:
-    "\<Gamma> \<turnstile> \<lparr>t1|;|fill \<delta>\<rparr> |:| A |\<times>| B \<Longrightarrow> \<Gamma> \<turnstile> \<lparr>\<pi>1 t1|;|fill \<delta>\<rparr> |:| A" |
+    "\<Gamma> \<turnstile> \<lparr>t1|;|fill \<sigma>\<rparr> |:| A |\<times>| B \<Longrightarrow> \<Gamma> \<turnstile> \<lparr>\<pi>1 t1|;|fill \<sigma>\<rparr> |:| A" |
   has_type_Proj2:
-    "\<Gamma> \<turnstile> \<lparr>t1|;|fill \<delta>\<rparr> |:| A |\<times>| B \<Longrightarrow> \<Gamma> \<turnstile> \<lparr>\<pi>2 t1|;|fill \<delta>\<rparr> |:| B" |
+    "\<Gamma> \<turnstile> \<lparr>t1|;|fill \<sigma>\<rparr> |:| A |\<times>| B \<Longrightarrow> \<Gamma> \<turnstile> \<lparr>\<pi>2 t1|;|fill \<sigma>\<rparr> |:| B" |
   has_type_Tuple:
-    "L\<noteq>[] \<Longrightarrow> length L = length TL \<Longrightarrow> (\<And>i. 0\<le>i \<Longrightarrow> i< length L \<Longrightarrow> \<Gamma> \<turnstile> \<lparr>(L ! i)|;|fill \<delta>\<rparr> |:| (TL ! i))
-      \<Longrightarrow> \<Gamma> \<turnstile> \<lparr>Tuple L|;|fill \<delta>\<rparr> |:| \<lparr>TL\<rparr>" |
+    "L\<noteq>[] \<Longrightarrow> length L = length TL \<Longrightarrow> (\<And>i. 0\<le>i \<Longrightarrow> i< length L \<Longrightarrow> \<Gamma> \<turnstile> \<lparr>(L ! i)|;|fill \<sigma>\<rparr> |:| (TL ! i))
+      \<Longrightarrow> \<Gamma> \<turnstile> \<lparr>Tuple L|;|fill \<sigma>\<rparr> |:| \<lparr>TL\<rparr>" |
   has_type_ProjT:
-    "1\<le>i \<Longrightarrow> i\<le> length TL \<Longrightarrow> \<Gamma> \<turnstile> \<lparr>t|;|fill \<delta>\<rparr> |:| \<lparr>TL\<rparr> \<Longrightarrow> \<Gamma> \<turnstile> \<lparr>\<Pi> i t|;|fill \<delta>\<rparr> |:| (TL ! (i-1))" |
+    "1\<le>i \<Longrightarrow> i\<le> length TL \<Longrightarrow> \<Gamma> \<turnstile> \<lparr>t|;|fill \<sigma>\<rparr> |:| \<lparr>TL\<rparr> \<Longrightarrow> \<Gamma> \<turnstile> \<lparr>\<Pi> i t|;|fill \<sigma>\<rparr> |:| (TL ! (i-1))" |
   has_type_RCD:
-    "L\<noteq>[] \<Longrightarrow> distinct L \<Longrightarrow> length LT = length TL \<Longrightarrow> length L = length LT \<Longrightarrow> (\<And>i. i< length LT \<Longrightarrow> \<Gamma> \<turnstile> \<lparr>(LT ! i)|;|fill \<delta>\<rparr> |:| (TL ! i))
-      \<Longrightarrow> \<Gamma> \<turnstile> \<lparr>Record L LT|;|fill \<delta>\<rparr> |:| \<lparr>L|:|TL\<rparr>" |
+    "L\<noteq>[] \<Longrightarrow> distinct L \<Longrightarrow> length LT = length TL \<Longrightarrow> length L = length LT \<Longrightarrow> (\<And>i. i< length LT \<Longrightarrow> \<Gamma> \<turnstile> \<lparr>(LT ! i)|;|fill \<sigma>\<rparr> |:| (TL ! i))
+      \<Longrightarrow> \<Gamma> \<turnstile> \<lparr>Record L LT|;|fill \<sigma>\<rparr> |:| \<lparr>L|:|TL\<rparr>" |
   has_type_ProjR:
-    "distinct L1 \<Longrightarrow> l\<in> set L1  \<Longrightarrow> length L1 = length TL \<Longrightarrow> \<Gamma> \<turnstile> \<lparr>t|;|fill \<delta>\<rparr> |:| \<lparr>L1|:|TL\<rparr> \<Longrightarrow> \<Gamma> \<turnstile> \<lparr>ProjR l t|;|fill \<delta>\<rparr> |:| (TL ! index L1 l)" |
+    "distinct L1 \<Longrightarrow> l\<in> set L1  \<Longrightarrow> length L1 = length TL \<Longrightarrow> \<Gamma> \<turnstile> \<lparr>t|;|fill \<sigma>\<rparr> |:| \<lparr>L1|:|TL\<rparr> \<Longrightarrow> \<Gamma> \<turnstile> \<lparr>ProjR l t|;|fill \<sigma>\<rparr> |:| (TL ! index L1 l)" |
   has_type_PatternVar:
-    "\<Gamma> \<turnstile> \<lparr> (fill \<delta>^^n) (<|V k|>) |;| id\<rparr> |:| A \<Longrightarrow>  set(patterns ((fill \<delta>^^n) (<|V k|>))) = {}\<Longrightarrow> \<Gamma> \<turnstile> \<lparr><|V k|>|;|fill \<delta>\<rparr> |:| A" |
+    "(\<And>\<sigma>1. \<Gamma> \<turnstile> \<lparr> (fill \<sigma>^^n) (<|V k|>) |;| fill \<sigma>1\<rparr> |:| A) \<Longrightarrow>  set(patterns ((fill \<sigma>^^n) (<|V k|>))) = {}\<Longrightarrow> \<Gamma> \<turnstile> \<lparr><|V k|>|;|fill \<sigma>\<rparr> |:| A" |
   has_type_PatternRCD:
-    "L\<noteq>[] \<Longrightarrow> distinct L \<Longrightarrow> length PL = length TL \<Longrightarrow> length L = length PL \<Longrightarrow> (\<And>i. i< length PL \<Longrightarrow> \<Gamma> \<turnstile> \<lparr><|PL ! i|>|;|fill \<delta>\<rparr> |:| (TL ! i))
-      \<Longrightarrow> \<Gamma> \<turnstile> \<lparr><|RCD L PL|>|;|fill \<delta>\<rparr> |:| \<lparr>L|:|TL\<rparr>" |
- (* has_type_LetPattern:
-    "coherent p \<Longrightarrow> Lmatch p t1 \<delta>  \<Longrightarrow> \<Gamma> \<turnstile> \<lparr>t1|;|fill \<delta>1\<rparr> |:| R \<Longrightarrow>
-     \<Gamma> \<turnstile> \<lparr>t2|;|((fill \<delta>1) \<circ> \<delta>)\<rparr> |:| A \<Longrightarrow> \<Gamma> \<turnstile> \<lparr>Let pattern p := t1 in t2|;|fill \<delta>1\<rparr> |:| A" |*)
+    "L\<noteq>[] \<Longrightarrow> distinct L \<Longrightarrow> length PL = length TL \<Longrightarrow> length L = length PL \<Longrightarrow> (\<And>i. i< length PL \<Longrightarrow> \<Gamma> \<turnstile> \<lparr><|PL ! i|>|;|fill \<sigma>\<rparr> |:| (TL ! i))
+      \<Longrightarrow> \<Gamma> \<turnstile> \<lparr><|RCD L PL|>|;|fill \<sigma>\<rparr> |:| \<lparr>L|:|TL\<rparr>" |
   has_type_LetPattern:
-    "coherent p \<Longrightarrow> Lmatch p t1 \<delta>  \<Longrightarrow> 
-     \<Gamma> \<turnstile> \<lparr>t2|;|((fill \<delta>1) \<circ> \<delta>)\<rparr> |:| A \<Longrightarrow> \<Gamma> \<turnstile> \<lparr>Let pattern p := t1 in t2|;|fill \<delta>1\<rparr> |:| A" |
+    "coherent p \<Longrightarrow> Lmatch p t1 \<sigma>  \<Longrightarrow> 
+     \<Gamma> \<turnstile> \<lparr>t2|;|((fill \<sigma>1) \<circ> \<sigma>)\<rparr> |:| A \<Longrightarrow> \<Gamma> \<turnstile> \<lparr>Let pattern p := t1 in t2|;|fill \<sigma>1\<rparr> |:| A" |
   has_type_Inl:
-    "\<Gamma> \<turnstile> \<lparr>t1|;|fill \<delta>1\<rparr> |:| A \<Longrightarrow> \<Gamma> \<turnstile> \<lparr>inl t1 as A|+|B |;|fill \<delta>1\<rparr> |:| A|+|B" |
+    "\<Gamma> \<turnstile> \<lparr>t1|;|fill \<sigma>1\<rparr> |:| A \<Longrightarrow> \<Gamma> \<turnstile> \<lparr>inl t1 as A|+|B |;|fill \<sigma>1\<rparr> |:| A|+|B" |
   has_type_Inr:
-    "\<Gamma> \<turnstile> \<lparr>t1|;|fill \<delta>1\<rparr> |:| B \<Longrightarrow> \<Gamma> \<turnstile> \<lparr>inr t1 as A|+|B |;|fill \<delta>1\<rparr> |:| A|+|B" |
+    "\<Gamma> \<turnstile> \<lparr>t1|;|fill \<sigma>1\<rparr> |:| B \<Longrightarrow> \<Gamma> \<turnstile> \<lparr>inr t1 as A|+|B |;|fill \<sigma>1\<rparr> |:| A|+|B" |
   has_type_Case:
-    "\<Gamma> \<turnstile> \<lparr> t|;|fill \<delta>1 \<rparr> |:| A|+|B \<Longrightarrow> replace x A \<Gamma> \<turnstile> \<lparr>t1|;|fill \<delta>1\<rparr> |:| C \<Longrightarrow>
-     replace y B \<Gamma> \<turnstile> \<lparr>t2|;|fill \<delta>1\<rparr> |:| C \<Longrightarrow> \<Gamma> \<turnstile> \<lparr>Case t of Inl x \<Rightarrow> t1 | Inr y \<Rightarrow> t2 |;|fill \<delta>1\<rparr> |:| C" |
+    "\<Gamma> \<turnstile> \<lparr> t|;|fill \<sigma>1 \<rparr> |:| A|+|B \<Longrightarrow> insert_nth x A \<Gamma> \<turnstile> \<lparr>t1|;|fill \<sigma>1\<rparr> |:| C \<Longrightarrow>
+     insert_nth y B \<Gamma> \<turnstile> \<lparr>t2|;|fill \<sigma>1\<rparr> |:| C \<Longrightarrow> \<Gamma> \<turnstile> \<lparr>Case t of Inl x \<Rightarrow> t1 | Inr y \<Rightarrow> t2 |;|fill \<sigma>1\<rparr> |:| C" |
   has_type_Variant:
-    "\<Gamma> \<turnstile> \<lparr> t |;| fill \<delta> \<rparr> |:| (TL!i) \<Longrightarrow> \<Gamma> \<turnstile> \<lparr> <(L!i):=t> as <L|,|TL> |;| fill \<delta> \<rparr> |:| <L|,|TL>" |
+    "\<Gamma> \<turnstile> \<lparr> t |;| fill \<sigma> \<rparr> |:| (TL!i) \<Longrightarrow> \<Gamma> \<turnstile> \<lparr> <(L!i):=t> as <L|,|TL> |;| fill \<sigma> \<rparr> |:| <L|,|TL>" |
   has_type_CaseV:
     " L\<noteq>\<emptyset> \<Longrightarrow> length I = length L \<Longrightarrow> length L = length TL \<Longrightarrow> length L = length LT \<Longrightarrow>
-      \<Gamma> \<turnstile> \<lparr> t |;| fill \<delta> \<rparr> |:| <L|,|TL> \<Longrightarrow> (\<forall>i<length L. replace (I!i) (TL!i) \<Gamma> \<turnstile> \<lparr>(LT!i)|;|fill \<delta>\<rparr> |:| A) \<Longrightarrow>
-      \<Gamma> \<turnstile> \<lparr> Case t of <L:=I> \<Rightarrow> LT |;|fill \<delta>\<rparr> |:| A" |
+      \<Gamma> \<turnstile> \<lparr> t |;| fill \<sigma> \<rparr> |:| <L|,|TL> \<Longrightarrow> (\<forall>i<length L. insert_nth (I!i) (TL!i) \<Gamma> \<turnstile> \<lparr>(LT!i)|;|fill \<sigma>\<rparr> |:| A) \<Longrightarrow>
+      \<Gamma> \<turnstile> \<lparr> Case t of <L:=I> \<Rightarrow> LT |;|fill \<sigma>\<rparr> |:| A" |
   has_type_Fix:
-    "\<Gamma> \<turnstile> \<lparr> t |;| fill \<delta> \<rparr> |:| A\<rightarrow>A \<Longrightarrow> \<Gamma> \<turnstile> \<lparr> fix t |;| fill \<delta> \<rparr> |:| A"
+    "\<Gamma> \<turnstile> \<lparr> t |;| fill \<sigma> \<rparr> |:| A\<rightarrow>A \<Longrightarrow> \<Gamma> \<turnstile> \<lparr> fix t |;| fill \<sigma> \<rparr> |:| A"
 
-inductive_cases has_type_LetE : "\<Gamma> \<turnstile> \<lparr> Let var x := t1 in t2|;|\<delta>1\<rparr>  |:| B"
-inductive_cases has_type_ProjTE: "\<Gamma> \<turnstile> \<lparr> \<Pi> i t|;|\<delta>1\<rparr> |:| R"
-inductive_cases has_type_ProjRE: "\<Gamma> \<turnstile> \<lparr> ProjR l t|;|\<delta>1\<rparr> |:| R"
-inductive_cases has_type_LetPE: "\<Gamma> \<turnstile> \<lparr>Let pattern p := t1 in t2|;|\<delta>1\<rparr> |:| A"
-inductive_cases has_type_CaseSE: "\<Gamma> \<turnstile> \<lparr>Case t of Inl x \<Rightarrow> t1 | Inr y \<Rightarrow> t2|;|\<delta>1\<rparr> |:| R"
-inductive_cases has_type_CaseVE: "\<Gamma> \<turnstile> \<lparr>Case t of <L:=I> \<Rightarrow> LT|;|\<delta>1\<rparr> |:| R"
-inductive_cases has_type_LAbsE: "\<Gamma> \<turnstile> \<lparr>LAbs T1 t2|;|fill \<delta>'\<rparr> |:| R"
-inductive_cases has_type_VariantE: "\<Gamma> \<turnstile> \<lparr><l:=t> as R |;|\<delta>1\<rparr> |:| R"
+inductive_cases has_type_LetE : "\<Gamma> \<turnstile> \<lparr> Let var x := t1 in t2|;|\<sigma>1\<rparr>  |:| B"
+inductive_cases has_type_ProjTE: "\<Gamma> \<turnstile> \<lparr> \<Pi> i t|;|\<sigma>1\<rparr> |:| R"
+inductive_cases has_type_ProjRE: "\<Gamma> \<turnstile> \<lparr> ProjR l t|;|\<sigma>1\<rparr> |:| R"
+inductive_cases has_type_LetPE: "\<Gamma> \<turnstile> \<lparr>Let pattern p := t1 in t2|;|\<sigma>1\<rparr> |:| A"
+inductive_cases has_type_CaseSE: "\<Gamma> \<turnstile> \<lparr>Case t of Inl x \<Rightarrow> t1 | Inr y \<Rightarrow> t2|;|\<sigma>1\<rparr> |:| R"
+inductive_cases has_type_CaseVE: "\<Gamma> \<turnstile> \<lparr>Case t of <L:=I> \<Rightarrow> LT|;|\<sigma>1\<rparr> |:| R"
+inductive_cases has_type_LAbsE: "\<Gamma> \<turnstile> \<lparr>LAbs T1 t2|;|fill \<sigma>'\<rparr> |:| R"
+inductive_cases has_type_VariantE: "\<Gamma> \<turnstile> \<lparr><l:=t> as R |;|\<sigma>1\<rparr> |:| R"
 
 lemma record_patterns_characterisation:
   "set (patterns (<|RCD L PL|>)) \<subseteq> S \<Longrightarrow> x \<in> set PL \<Longrightarrow> set(patterns (<|x|>)) \<subseteq> S"
 by (induction PL arbitrary: S x, auto) 
 
 lemma inversion:
-  "\<Gamma> \<turnstile> \<lparr> LTrue |;| \<delta>\<rparr> |:| R \<Longrightarrow> R = Bool"
-  "\<Gamma> \<turnstile> \<lparr> LFalse |;| \<delta>\<rparr> |:| R \<Longrightarrow> R = Bool"
-  "\<Gamma> \<turnstile> \<lparr> LIf t1 t2 t3 |;| \<delta>\<rparr> |:| R \<Longrightarrow>  \<Gamma> \<turnstile> \<lparr>t1|;| \<delta>\<rparr> |:| Bool \<and> \<Gamma> \<turnstile> \<lparr>t2|;| \<delta>\<rparr> |:| R \<and> \<Gamma> \<turnstile> \<lparr>t3|;| \<delta>\<rparr> |:| R"
-  "\<Gamma> \<turnstile> \<lparr> LVar x|;| \<delta>\<rparr> |:| R \<Longrightarrow> (x, R) |\<in>| \<Gamma>"
-  "\<Gamma> \<turnstile> \<lparr> LAbs T1 t2 |;| fill \<delta>'\<rparr> |:| R \<Longrightarrow> \<exists>R2. R = T1 \<rightarrow> R2 \<and>  \<Gamma> |,| T1 \<turnstile> \<lparr>t2|;|fill \<delta>'\<rparr> |:| R2 "
-  "\<Gamma> \<turnstile> \<lparr> LApp t1 t2 |;| \<delta>\<rparr> |:| R \<Longrightarrow> \<exists>T11. \<Gamma> \<turnstile> \<lparr>t1|;| \<delta>\<rparr> |:| T11 \<rightarrow> R \<and> \<Gamma> \<turnstile> \<lparr>t2|;| \<delta>\<rparr> |:| T11"
-  "\<Gamma> \<turnstile> \<lparr> unit|;| \<delta>\<rparr> |:| R \<Longrightarrow> R = Unit"
-  "\<Gamma> \<turnstile> \<lparr> Seq t1 t2 |;| \<delta>\<rparr> |:| R \<Longrightarrow> \<exists>A. R = A \<and> \<Gamma> \<turnstile> \<lparr>t2|;| \<delta>\<rparr> |:| A \<and> \<Gamma> \<turnstile> \<lparr>t1|;| \<delta>\<rparr> |:| Unit"
-  "\<Gamma> \<turnstile> \<lparr> t as A |;| \<delta>\<rparr> |:| R \<Longrightarrow> R = A"
-  "\<Gamma> \<turnstile> \<lparr> Let var x := t in t1 |;| \<delta>\<rparr> |:| R \<Longrightarrow> \<exists>A B. R = B \<and> \<Gamma> \<turnstile> \<lparr> t|;| \<delta>\<rparr> |:| A \<and> (insert_nth x A \<Gamma>) \<turnstile> \<lparr>shift_L 1 x t1|;| \<delta>\<rparr> |:| B"
-  "\<Gamma> \<turnstile> \<lparr> \<lbrace>t1,t2\<rbrace>|;| \<delta>\<rparr> |:| R \<Longrightarrow> \<exists>A B. \<Gamma> \<turnstile> \<lparr> t1|;| \<delta>\<rparr> |:| A \<and> \<Gamma> \<turnstile> \<lparr> t2|;| \<delta>\<rparr> |:| B \<and> R = A |\<times>| B"
-  "\<Gamma> \<turnstile> \<lparr> \<pi>1 t|;| \<delta>\<rparr> |:| R \<Longrightarrow> \<exists>A B. \<Gamma> \<turnstile> \<lparr> t|;| \<delta>\<rparr> |:| A |\<times>| B \<and> R = A"
-  "\<Gamma> \<turnstile> \<lparr> \<pi>2 t|;| \<delta>\<rparr> |:| R \<Longrightarrow> \<exists>A B. \<Gamma> \<turnstile> \<lparr> t|;| \<delta>\<rparr> |:| A |\<times>| B \<and> R = B"
-  "\<Gamma> \<turnstile> \<lparr> Tuple L|;| \<delta>\<rparr> |:| R \<Longrightarrow> \<exists>TL. length L = length TL \<and> (\<forall>i. 0\<le>i \<longrightarrow> i< length L \<longrightarrow> \<Gamma> \<turnstile> \<lparr>(L ! i)|;| \<delta>\<rparr> |:| (TL ! i)) \<and> R = \<lparr>TL\<rparr>"
-  "\<Gamma> \<turnstile> \<lparr> (\<Pi> i t)|;| \<delta>\<rparr> |:| R \<Longrightarrow> \<exists>TL. R = (TL ! (i-1)) \<and> \<Gamma> \<turnstile> \<lparr>t|;| \<delta>\<rparr> |:| \<lparr>TL\<rparr> \<and> 1\<le>i \<and> i\<le> length TL"
-  "\<Gamma> \<turnstile> \<lparr> (Record L1 LT)|;| \<delta>\<rparr> |:| R \<Longrightarrow> \<exists>TL. R = \<lparr>L1|:|TL\<rparr> \<and> length TL = length LT \<and> length L1 = length LT \<and> distinct L1 \<and> 
-                                    (\<forall>i. 0\<le>i \<longrightarrow> i< length LT \<longrightarrow> \<Gamma> \<turnstile> \<lparr> (LT ! i)|;| \<delta>\<rparr> |:| (TL ! i)) " 
-  "\<Gamma> \<turnstile> \<lparr> (ProjR l t)|;| \<delta>\<rparr> |:| R \<Longrightarrow>\<exists>m L TL. \<Gamma> \<turnstile> \<lparr>t |;| \<delta>\<rparr> |:| \<lparr>L|:|TL\<rparr> \<and> index L l = m \<and> TL ! m = R \<and> distinct L \<and> length L = length TL
+  "\<Gamma> \<turnstile> \<lparr> LTrue |;| \<sigma>\<rparr> |:| R \<Longrightarrow> R = Bool"
+  "\<Gamma> \<turnstile> \<lparr> LFalse |;| \<sigma>\<rparr> |:| R \<Longrightarrow> R = Bool"
+  "\<Gamma> \<turnstile> \<lparr> LIf t1 t2 t3 |;| \<sigma>\<rparr> |:| R \<Longrightarrow>  \<Gamma> \<turnstile> \<lparr>t1|;| \<sigma>\<rparr> |:| Bool \<and> \<Gamma> \<turnstile> \<lparr>t2|;| \<sigma>\<rparr> |:| R \<and> \<Gamma> \<turnstile> \<lparr>t3|;| \<sigma>\<rparr> |:| R"
+  "\<Gamma> \<turnstile> \<lparr> LVar x|;| \<sigma>\<rparr> |:| R \<Longrightarrow> (x, R) |\<in>| \<Gamma>"
+  "\<Gamma> \<turnstile> \<lparr> LAbs T1 t2 |;| fill \<sigma>'\<rparr> |:| R \<Longrightarrow> \<exists>R2. R = T1 \<rightarrow> R2 \<and>  \<Gamma> |,| T1 \<turnstile> \<lparr>t2|;|fill \<sigma>'\<rparr> |:| R2 "
+  "\<Gamma> \<turnstile> \<lparr> LApp t1 t2 |;| \<sigma>\<rparr> |:| R \<Longrightarrow> \<exists>T11. \<Gamma> \<turnstile> \<lparr>t1|;| \<sigma>\<rparr> |:| T11 \<rightarrow> R \<and> \<Gamma> \<turnstile> \<lparr>t2|;| \<sigma>\<rparr> |:| T11"
+  "\<Gamma> \<turnstile> \<lparr> unit|;| \<sigma>\<rparr> |:| R \<Longrightarrow> R = Unit"
+  "\<Gamma> \<turnstile> \<lparr> Seq t1 t2 |;| \<sigma>\<rparr> |:| R \<Longrightarrow> \<exists>A. R = A \<and> \<Gamma> \<turnstile> \<lparr>t2|;| \<sigma>\<rparr> |:| A \<and> \<Gamma> \<turnstile> \<lparr>t1|;| \<sigma>\<rparr> |:| Unit"
+  "\<Gamma> \<turnstile> \<lparr> t as A |;| \<sigma>\<rparr> |:| R \<Longrightarrow> R = A"
+  "\<Gamma> \<turnstile> \<lparr> Let var x := t in t1 |;| \<sigma>\<rparr> |:| R \<Longrightarrow> \<exists>A B. R = B \<and> \<Gamma> \<turnstile> \<lparr> t|;| \<sigma>\<rparr> |:| A \<and> (insert_nth x A \<Gamma>) \<turnstile> \<lparr>t1|;| \<sigma>\<rparr> |:| B"
+  "\<Gamma> \<turnstile> \<lparr> \<lbrace>t1,t2\<rbrace>|;| \<sigma>\<rparr> |:| R \<Longrightarrow> \<exists>A B. \<Gamma> \<turnstile> \<lparr> t1|;| \<sigma>\<rparr> |:| A \<and> \<Gamma> \<turnstile> \<lparr> t2|;| \<sigma>\<rparr> |:| B \<and> R = A |\<times>| B"
+  "\<Gamma> \<turnstile> \<lparr> \<pi>1 t|;| \<sigma>\<rparr> |:| R \<Longrightarrow> \<exists>A B. \<Gamma> \<turnstile> \<lparr> t|;| \<sigma>\<rparr> |:| A |\<times>| B \<and> R = A"
+  "\<Gamma> \<turnstile> \<lparr> \<pi>2 t|;| \<sigma>\<rparr> |:| R \<Longrightarrow> \<exists>A B. \<Gamma> \<turnstile> \<lparr> t|;| \<sigma>\<rparr> |:| A |\<times>| B \<and> R = B"
+  "\<Gamma> \<turnstile> \<lparr> Tuple L|;| \<sigma>\<rparr> |:| R \<Longrightarrow> \<exists>TL. length L = length TL \<and> (\<forall>i. 0\<le>i \<longrightarrow> i< length L \<longrightarrow> \<Gamma> \<turnstile> \<lparr>(L ! i)|;| \<sigma>\<rparr> |:| (TL ! i)) \<and> R = \<lparr>TL\<rparr>"
+  "\<Gamma> \<turnstile> \<lparr> (\<Pi> i t)|;| \<sigma>\<rparr> |:| R \<Longrightarrow> \<exists>TL. R = (TL ! (i-1)) \<and> \<Gamma> \<turnstile> \<lparr>t|;| \<sigma>\<rparr> |:| \<lparr>TL\<rparr> \<and> 1\<le>i \<and> i\<le> length TL"
+  "\<Gamma> \<turnstile> \<lparr> (Record L1 LT)|;| \<sigma>\<rparr> |:| R \<Longrightarrow> \<exists>TL. R = \<lparr>L1|:|TL\<rparr> \<and> length TL = length LT \<and> length L1 = length LT \<and> distinct L1 \<and> 
+                                    (\<forall>i. 0\<le>i \<longrightarrow> i< length LT \<longrightarrow> \<Gamma> \<turnstile> \<lparr> (LT ! i)|;| \<sigma>\<rparr> |:| (TL ! i)) " 
+  "\<Gamma> \<turnstile> \<lparr> (ProjR l t)|;| \<sigma>\<rparr> |:| R \<Longrightarrow>\<exists>m L TL. \<Gamma> \<turnstile> \<lparr>t |;| \<sigma>\<rparr> |:| \<lparr>L|:|TL\<rparr> \<and> index L l = m \<and> TL ! m = R \<and> distinct L \<and> length L = length TL
                               \<and> l \<in> set L"
-  "\<Gamma> \<turnstile> \<lparr><|V k|>|;|\<delta>\<rparr> |:| R \<Longrightarrow> \<exists>n. \<Gamma> \<turnstile> \<lparr>(\<delta>^^n) (<|V k|>)|;| id\<rparr> |:| R \<and>  set(patterns ((\<delta>^^n) (<|V k|>))) = {}"
-  "\<Gamma> \<turnstile> \<lparr><|RCD L1 PL|>|;|\<delta>\<rparr> |:| R \<Longrightarrow> \<exists>TL. R = \<lparr>L1|:|TL\<rparr> \<and> L1\<noteq>[] \<and> distinct L1 \<and> length PL = length TL \<and> length L1 = length PL \<and>
-                                    (\<forall>i< length PL. \<Gamma> \<turnstile> \<lparr><|PL ! i|>|;|\<delta>\<rparr> |:| (TL ! i))"
-  "\<Gamma> \<turnstile> \<lparr>Let pattern p := t1 in t2|;|\<delta>1\<rparr> |:| R \<Longrightarrow>\<exists>\<delta>. coherent p \<and> Lmatch p t1 \<delta>  \<and> \<Gamma> \<turnstile> \<lparr>t2|;|(\<delta>1 \<circ> \<delta>)\<rparr> |:| R" 
-  "\<Gamma> \<turnstile> \<lparr>inl t as R|;|\<delta>1\<rparr> |:| R \<Longrightarrow>\<exists>A B. R = A|+|B \<and> \<Gamma> \<turnstile> \<lparr>t|;|\<delta>1\<rparr> |:| A"
-  "\<Gamma> \<turnstile> \<lparr>inr t as R|;|\<delta>1\<rparr> |:| R \<Longrightarrow>\<exists>A B. R = A|+|B \<and> \<Gamma> \<turnstile> \<lparr>t|;|\<delta>1\<rparr> |:| B"
-  "\<Gamma> \<turnstile> \<lparr>Case t of Inl x \<Rightarrow> t1 | Inr y \<Rightarrow> t2|;|\<delta>1\<rparr> |:| R \<Longrightarrow>\<exists>A B C. R = C \<and> \<Gamma> \<turnstile> \<lparr>t|;|\<delta>1\<rparr> |:| A|+|B \<and>
-                                                          replace x A \<Gamma> \<turnstile> \<lparr>t1|;|\<delta>1\<rparr> |:| C \<and> replace y B \<Gamma> \<turnstile> \<lparr>t2|;|\<delta>1\<rparr> |:| C"
-   "\<Gamma> \<turnstile> \<lparr> <l:=t> as R |;| \<delta>1 \<rparr> |:| R \<Longrightarrow>\<exists>L TL i. R=<L|,|TL> \<and> \<Gamma> \<turnstile> \<lparr> t |;| \<delta>1 \<rparr> |:| (TL!i) \<and> l = L!i " 
-    " \<Gamma> \<turnstile> \<lparr> Case t of <L1:=I> \<Rightarrow> LT |;| \<delta>1\<rparr> |:| A \<Longrightarrow>\<exists>TL. L1\<noteq>\<emptyset> \<and> length I = length L1 \<and> length L1 = length TL \<and> length L1 = length LT \<and>
-      \<Gamma> \<turnstile> \<lparr> t |;| \<delta>1 \<rparr> |:| <L1|,|TL> \<and> (\<forall>i<length L1. replace (I!i) (TL!i) \<Gamma> \<turnstile> \<lparr>(LT!i)|;| \<delta>1\<rparr> |:| A)"
+  "\<Gamma> \<turnstile> \<lparr><|V k|>|;|\<sigma>\<rparr> |:| R \<Longrightarrow> \<exists>n. (\<forall>\<sigma>1. \<Gamma> \<turnstile> \<lparr>(\<sigma>^^n) (<|V k|>)|;| fill \<sigma>1\<rparr> |:| R) \<and>  set(patterns ((\<sigma>^^n) (<|V k|>))) = {}"
+  "\<Gamma> \<turnstile> \<lparr><|RCD L1 PL|>|;|\<sigma>\<rparr> |:| R \<Longrightarrow> \<exists>TL. R = \<lparr>L1|:|TL\<rparr> \<and> L1\<noteq>[] \<and> distinct L1 \<and> length PL = length TL \<and> length L1 = length PL \<and>
+                                    (\<forall>i< length PL. \<Gamma> \<turnstile> \<lparr><|PL ! i|>|;|\<sigma>\<rparr> |:| (TL ! i))"
+  "\<Gamma> \<turnstile> \<lparr>Let pattern p := t1 in t2|;|\<sigma>1\<rparr> |:| R \<Longrightarrow>\<exists>\<sigma>. coherent p \<and> Lmatch p t1 \<sigma>  \<and> \<Gamma> \<turnstile> \<lparr>t2|;|(\<sigma>1 \<circ> \<sigma>)\<rparr> |:| R" 
+  "\<Gamma> \<turnstile> \<lparr>inl t as R|;|\<sigma>1\<rparr> |:| R \<Longrightarrow>\<exists>A B. R = A|+|B \<and> \<Gamma> \<turnstile> \<lparr>t|;|\<sigma>1\<rparr> |:| A"
+  "\<Gamma> \<turnstile> \<lparr>inr t as R|;|\<sigma>1\<rparr> |:| R \<Longrightarrow>\<exists>A B. R = A|+|B \<and> \<Gamma> \<turnstile> \<lparr>t|;|\<sigma>1\<rparr> |:| B"
+  "\<Gamma> \<turnstile> \<lparr>Case t of Inl x \<Rightarrow> t1 | Inr y \<Rightarrow> t2|;|\<sigma>1\<rparr> |:| R \<Longrightarrow>\<exists>A B C. R = C \<and> \<Gamma> \<turnstile> \<lparr>t|;|\<sigma>1\<rparr> |:| A|+|B \<and>
+                                                          insert_nth x A \<Gamma> \<turnstile> \<lparr>t1|;|\<sigma>1\<rparr> |:| C \<and> insert_nth y B \<Gamma> \<turnstile> \<lparr>t2|;|\<sigma>1\<rparr> |:| C"
+   "\<Gamma> \<turnstile> \<lparr> <l:=t> as R |;| \<sigma>1 \<rparr> |:| R \<Longrightarrow>\<exists>L TL i. R=<L|,|TL> \<and> \<Gamma> \<turnstile> \<lparr> t |;| \<sigma>1 \<rparr> |:| (TL!i) \<and> l = L!i " 
+    " \<Gamma> \<turnstile> \<lparr> Case t of <L1:=I> \<Rightarrow> LT |;| \<sigma>1\<rparr> |:| A \<Longrightarrow>\<exists>TL. L1\<noteq>\<emptyset> \<and> length I = length L1 \<and> length L1 = length TL \<and> length L1 = length LT \<and>
+      \<Gamma> \<turnstile> \<lparr> t |;| \<sigma>1 \<rparr> |:| <L1|,|TL> \<and> (\<forall>i<length L1. insert_nth (I!i) (TL!i) \<Gamma> \<turnstile> \<lparr>(LT!i)|;| \<sigma>1\<rparr> |:| A)"
 proof -
-  assume H:"\<Gamma> \<turnstile> \<lparr> Let var x := t in t1|;|\<delta>\<rparr> |:| R"
-  show "\<exists>A B. R = B \<and> \<Gamma> \<turnstile> \<lparr>t|;|\<delta>\<rparr> |:| A \<and> insert_nth x A \<Gamma> \<turnstile> \<lparr>shift_L 1 x t1|;|\<delta>\<rparr> |:| B"
-    using H has_type_LetE
-    by (cases "x\<ge> length \<Gamma>", fastforce+)
+  assume H:"\<Gamma> \<turnstile> \<lparr> Let var x := t in t1|;|\<sigma>\<rparr> |:| R"
+  show " \<exists>A B. R = B \<and> \<Gamma> \<turnstile> \<lparr> t|;| \<sigma>\<rparr> |:| A \<and> (insert_nth x A \<Gamma>) \<turnstile> \<lparr>t1|;| \<sigma>\<rparr> |:| B"
+    using has_type_LetE[OF H] 
+    by fastforce 
 next
-  assume H1: "\<Gamma> \<turnstile> \<lparr>Let pattern p := t1 in t2|;|\<delta>1\<rparr> |:| R"
-  show "\<exists>\<delta>. coherent p \<and> Lmatch p t1 \<delta>  \<and> \<Gamma> \<turnstile> \<lparr>t2|;|(\<delta>1 \<circ> \<delta>)\<rparr> |:| R"
+  assume H:"\<Gamma> \<turnstile> \<lparr><|V k|>|;|\<sigma>\<rparr> |:| R"
+  show "\<exists>n. (\<forall>\<sigma>1. \<Gamma> \<turnstile> \<lparr>(\<sigma>^^n) (<|V k|>)|;| fill \<sigma>1\<rparr> |:| R) \<and>  set(patterns ((\<sigma>^^n) (<|V k|>))) = {}"
+    using H[unfolded has_type_L.simps[of \<Gamma>], simplified]
+    by blast
+next
+  assume H1: "\<Gamma> \<turnstile> \<lparr>Let pattern p := t1 in t2|;|\<sigma>1\<rparr> |:| R"
+  show "\<exists>\<sigma>. coherent p \<and> Lmatch p t1 \<sigma>  \<and> \<Gamma> \<turnstile> \<lparr>t2|;|(\<sigma>1 \<circ> \<sigma>)\<rparr> |:| R"
     using has_type_LetPE[OF H1]
     by metis
 next
-  assume H2: "\<Gamma> \<turnstile> \<lparr>Case t of Inl x \<Rightarrow> t1 | Inr y \<Rightarrow> t2|;|\<delta>1\<rparr> |:| R"
-  show "\<exists>A B C. R = C \<and> \<Gamma> \<turnstile> \<lparr>t|;|\<delta>1\<rparr> |:| A |+| B \<and> replace x A \<Gamma> \<turnstile> \<lparr>t1|;|\<delta>1\<rparr> |:| C \<and> replace y B \<Gamma> \<turnstile> \<lparr>t2|;|\<delta>1\<rparr> |:| C"
-    by (cases "length \<Gamma> \<le> x"; cases "length \<Gamma> \<le> y"; insert has_type_CaseSE[OF H2]; metis (full_types) replace.simps)
+  assume H2: "\<Gamma> \<turnstile> \<lparr>Case t of Inl x \<Rightarrow> t1 | Inr y \<Rightarrow> t2|;|\<sigma>1\<rparr> |:| R"
+  show "\<exists>A B C. R = C \<and> \<Gamma> \<turnstile> \<lparr>t|;|\<sigma>1\<rparr> |:| A |+| B \<and> insert_nth x A \<Gamma> \<turnstile> \<lparr>t1|;|\<sigma>1\<rparr> |:| C \<and> insert_nth y B \<Gamma> \<turnstile> \<lparr>t2|;|\<sigma>1\<rparr> |:| C"
+    using has_type_CaseSE[OF H2]
+    by fastforce
 next
-  assume H4: "\<Gamma> \<turnstile> \<lparr><l:=t> as R|;|\<delta>1\<rparr> |:| R"
-  show  "\<exists>L TL i. R = <L|,|TL> \<and> \<Gamma> \<turnstile> \<lparr>t|;|\<delta>1\<rparr> |:| (TL ! i) \<and> l = L ! i"
+  assume H4: "\<Gamma> \<turnstile> \<lparr><l:=t> as R|;|\<sigma>1\<rparr> |:| R"
+  show  "\<exists>L TL i. R = <L|,|TL> \<and> \<Gamma> \<turnstile> \<lparr>t|;|\<sigma>1\<rparr> |:| (TL ! i) \<and> l = L ! i"
     using has_type_VariantE[OF H4]
     by metis    
 next
-  assume H5: "\<Gamma> \<turnstile> \<lparr>Case t of <L1:=I> \<Rightarrow> LT|;|\<delta>1\<rparr> |:| A"
-  have "\<And>TL \<delta>. \<delta>1 = fill \<delta> \<Longrightarrow> length L1 = length TL \<Longrightarrow>\<forall>i<length TL. (if length \<Gamma> \<le> I ! i then \<Gamma> else take (I ! i) \<Gamma> @ \<emptyset> |,| (TL ! i) @ drop (Suc (I ! i)) \<Gamma>) \<turnstile> \<lparr>(LT ! i)|;|fill \<delta>\<rparr> |:| A
-         \<Longrightarrow> \<forall>i<length L1. replace (I ! i) (TL ! i) \<Gamma> \<turnstile> \<lparr>(LT ! i)|;|\<delta>1\<rparr> |:| A"
+  assume H5: "\<Gamma> \<turnstile> \<lparr>Case t of <L1:=I> \<Rightarrow> LT|;|\<sigma>1\<rparr> |:| A"
+  have "\<And>TL \<sigma>. \<sigma>1 = fill \<sigma> \<Longrightarrow> length L1 = length TL \<Longrightarrow>\<forall>i<length TL. (take (I ! i) \<Gamma> @ \<emptyset> |,| (TL ! i) @ drop (I ! i) \<Gamma>) \<turnstile> \<lparr>(LT ! i)|;|fill \<sigma>\<rparr> |:| A
+         \<Longrightarrow> \<forall>i<length L1. insert_nth (I ! i) (TL ! i) \<Gamma> \<turnstile> \<lparr>(LT ! i)|;|\<sigma>1\<rparr> |:| A"
     proof (rule+)
-      fix TL \<delta> i
-      assume hyps:"\<forall>i<length TL. (if length \<Gamma> \<le> I ! i then \<Gamma> else take (I ! i) \<Gamma> @ \<emptyset> |,| (TL ! i) @ drop (Suc (I ! i)) \<Gamma>) \<turnstile> \<lparr>(LT ! i)|;|fill \<delta>\<rparr> |:| A"
-                  "\<delta>1 = fill \<delta>" "i<length L1" "length L1 = length TL"
-      then show "replace (I ! i) (TL ! i) \<Gamma> \<turnstile> \<lparr>(LT ! i)|;|\<delta>1\<rparr> |:| A"
-        by (cases "length \<Gamma>\<le> I!i", fastforce+)
+      fix TL \<sigma> i
+      assume hyps:"\<forall>i<length TL. (take (I ! i) \<Gamma> @ \<emptyset> |,| (TL ! i) @ drop (I ! i) \<Gamma>) \<turnstile> \<lparr>(LT ! i)|;|fill \<sigma>\<rparr> |:| A"
+                  "\<sigma>1 = fill \<sigma>" "i<length L1" "length L1 = length TL"
+      then show "insert_nth (I ! i) (TL ! i) \<Gamma> \<turnstile> \<lparr>(LT ! i)|;|\<sigma>1\<rparr> |:| A"
+        by fastforce  
     qed      
-  then show "\<exists>TL. L1 \<noteq> \<emptyset> \<and> length I = length L1 \<and> length L1 = length TL \<and> length L1 = length LT \<and> 
-          \<Gamma> \<turnstile> \<lparr>t|;|\<delta>1\<rparr> |:| <L1|,|TL> \<and> (\<forall>i<length L1. replace (I ! i) (TL ! i) \<Gamma> \<turnstile> \<lparr>(LT ! i)|;|\<delta>1\<rparr> |:| A)"
+  then show "\<exists>TL. L1\<noteq>\<emptyset> \<and> length I = length L1 \<and> length L1 = length TL \<and> length L1 = length LT \<and>
+      \<Gamma> \<turnstile> \<lparr> t |;| \<sigma>1 \<rparr> |:| <L1|,|TL> \<and> (\<forall>i<length L1. insert_nth (I!i) (TL!i) \<Gamma> \<turnstile> \<lparr>(LT!i)|;| \<sigma>1\<rparr> |:| A)"
     using has_type_CaseVE[OF H5]
-    by metis
+    by (metis append_Cons append_Nil insert_nth_take_drop)
 qed (auto elim: has_type_L.cases has_type_ProjTE, metis has_type_ProjRE)
 
 
@@ -329,11 +332,11 @@ proof
 qed
 
 lemma fill_fill_comp:
-  "fill \<delta> \<circ> fill \<delta>1 = fill (fill \<delta> \<circ> \<delta>1)"
+  "fill \<sigma> \<circ> fill \<sigma>1 = fill (fill \<sigma> \<circ> \<sigma>1)"
 proof (rule)
   fix x
-  show "(fill \<delta> \<circ> fill \<delta>1) x= fill (fill \<delta> \<circ> \<delta>1) x"
-    proof (induction x arbitrary: \<delta> \<delta>1)
+  show "(fill \<sigma> \<circ> fill \<sigma>1) x= fill (fill \<sigma> \<circ> \<sigma>1) x"
+    proof (induction x arbitrary: \<sigma> \<sigma>1)
       case (Pattern p)
         show ?case
           proof (induction p)
@@ -347,7 +350,7 @@ proof (rule)
 qed
 
 lemma lmatch_gives_fill:
-  "Lmatch p t \<delta> \<Longrightarrow> \<exists>\<delta>1. fill \<delta>1 = \<delta>" 
+  "Lmatch p t \<sigma> \<Longrightarrow> \<exists>\<sigma>1. fill \<sigma>1 = \<sigma>" 
 proof (induction rule: Lmatch.induct)
   case (M_RCD L LT F PL)
     show ?case
@@ -365,17 +368,17 @@ proof (induction rule: Lmatch.induct)
           then obtain \<Delta> where BigCirc_\<Delta>:"fill \<Delta> = \<Odot> F"
             using Cons(1)[of PL'] Cons(2) Cons(3)[of "_+1"]
             by force
-          obtain \<delta>1 where "fill \<delta>1 = f"
+          obtain \<sigma>1 where "fill \<sigma>1 = f"
             using Cons(3)[of 0] Cons(2)
             by force
           with BigCirc_\<Delta> show ?case
-            using fill_fill_comp[of \<delta>1 \<Delta>]
+            using fill_fill_comp[of \<sigma>1 \<Delta>]
             by fastforce
       qed 
 qed auto
 
 lemma pattern_fill_shift:
-  "patterns ((fill (shift_L d c \<circ> \<delta>) ^^n) t) = patterns ((fill \<delta> ^^ n) t)"
+  "patterns ((fill (shift_L d c \<circ> \<sigma>) ^^n) t) = patterns ((fill \<sigma> ^^ n) t)"
 proof (induction n)
   case (Suc n1)
     show ?case
@@ -384,10 +387,10 @@ qed auto
 
 
 (*lemma weakening1 :
-  fixes \<Gamma>::lcontext  and t::lterm and A R::ltype and \<delta> \<delta>'::"nat\<Rightarrow>lterm"
-  assumes well_typed: "\<Gamma> \<turnstile> \<lparr>t|;|fill \<delta>\<rparr> |:| A" and
-          shifted_filling:"p\<in>set (patterns t) \<Longrightarrow> \<Gamma> \<turnstile> \<lparr><|V p|>|;|fill \<delta>\<rparr> |:| R \<Longrightarrow> \<Gamma> \<turnstile> \<lparr><|V p|>|;|fill \<delta>'\<rparr> |:| R"
-  shows "\<Gamma> \<turnstile> \<lparr>t |;| fill \<delta>'\<rparr> |:| A"
+  fixes \<Gamma>::lcontext  and t::lterm and A R::ltype and \<sigma> \<sigma>'::"nat\<Rightarrow>lterm"
+  assumes well_typed: "\<Gamma> \<turnstile> \<lparr>t|;|fill \<sigma>\<rparr> |:| A" and
+          shifted_filling:"p\<in>set (patterns t) \<Longrightarrow> \<Gamma> \<turnstile> \<lparr><|V p|>|;|fill \<sigma>\<rparr> |:| R \<Longrightarrow> \<Gamma> \<turnstile> \<lparr><|V p|>|;|fill \<sigma>'\<rparr> |:| R"
+  shows "\<Gamma> \<turnstile> \<lparr>t |;| fill \<sigma>'\<rparr> |:| A"
 sorry*)
 
 
@@ -395,79 +398,66 @@ sorry*)
 thm subst_L.cases[of "(j,s,LTrue)", simplified prod.inject "lterm.distinct" HOL.simp_thms HOL.False_implies_equals
   Pure.triv_forall_equality HOL.True_implies_equals]
 
-(*lemma P_set_Pat: 
-  "(\<And>x. x\<in>set(patterns t) \<Longrightarrow> P x) \<Longrightarrow> t'\<in> subterms t \<Longrightarrow> (\<And>x. x\<in>set(patterns t') \<Longrightarrow> P x)"
-proof (induction t)
-  case (LIf)
-    show ?case using LIf(4,5,6) by (simp; blast)      
-next
-  case (LetP)
-    show ?case using LetP(3,4,5) by (simp; blast)
-next
-  case (CaseSum)
-    show ?case using CaseSum(4,5,6) by (simp; blast)
-qed (simp; blast)+
-*)
 lemma P_list_conv_nth:"(\<And>x. x\<in> A\<union>set L \<Longrightarrow> P x) \<Longrightarrow> (\<And>i. i<length L \<Longrightarrow> P (L!i))"
 using set_conv_nth by auto
 
-
-
 lemma weakening :
-  fixes \<Gamma>::lcontext  and t::lterm and A S::ltype and \<delta> \<delta>'::"nat\<Rightarrow>lterm" and n::nat
-  assumes well_typed: "\<Gamma> \<turnstile> \<lparr>t|;|fill \<delta>\<rparr> |:| A" and
+  fixes \<Gamma>::lcontext  and t::lterm and A S::ltype and \<sigma> \<sigma>'::"nat\<Rightarrow>lterm" and n::nat
+  assumes well_typed: "\<Gamma> \<turnstile> \<lparr>t|;|fill \<sigma>\<rparr> |:| A" and
           weaker_ctx: " n \<le> length \<Gamma>" and
-          shifted_filling:"\<And>p R n. p\<in>set (patterns t) \<Longrightarrow> \<Gamma>' \<turnstile> \<lparr><|V p|>|;|fill \<delta>\<rparr> |:| R \<Longrightarrow> insert_nth n S \<Gamma>' \<turnstile> \<lparr><|V p|>|;|fill \<delta>'\<rparr> |:| R"
-  shows "insert_nth n S \<Gamma> \<turnstile> \<lparr>shift_L 1 n t|;|fill \<delta>'\<rparr> |:| A"
+          shifted_filling:"\<And>p R n. p\<in>set (patterns t) \<Longrightarrow> \<Gamma>' \<turnstile> \<lparr><|V p|>|;|fill \<sigma>\<rparr> |:| R \<Longrightarrow> insert_nth n S \<Gamma>' \<turnstile> \<lparr><|V p|>|;|fill \<sigma>'\<rparr> |:| R"
+  shows "insert_nth n S \<Gamma> \<turnstile> \<lparr>shift_L 1 n t|;|fill \<sigma>'\<rparr> |:| A"
 using assms 
-proof(induction \<Gamma> t "fill \<delta>" A arbitrary: n \<delta>' \<Gamma>' rule:has_type_L.induct)
-  case (has_type_LIf \<Gamma> t1 \<delta>1 t2 A t3)
+proof(induction \<Gamma> t "fill \<sigma>" A arbitrary: n \<sigma> \<sigma>' \<Gamma>' rule:has_type_L.induct)
+  case (has_type_LIf \<Gamma> t1 \<sigma>1 t2 A t3)
     show ?case
-      apply (insert P_pat_subterm_cases[where P="\<lambda>pt. (\<forall> x R n. x\<in>set pt \<longrightarrow> \<Gamma>' \<turnstile> \<lparr><|V x|>|;|fill \<delta>\<rparr> |:| R \<longrightarrow> insert_nth n S \<Gamma>' \<turnstile> \<lparr><|V x|>|;|fill \<delta>'\<rparr> |:| R)"
-                                and t="LIf t1 t2 t3", unfolded subterms.simps,  
+      apply (insert P_pat_subterm_cases[where P="\<lambda>pt. (\<forall> x R n. x\<in>set pt \<longrightarrow> \<Gamma>' \<turnstile> \<lparr><|V x|>|;|fill \<sigma>\<rparr> |:| R \<longrightarrow> insert_nth n S \<Gamma>' \<turnstile> \<lparr><|V x|>|;|fill \<sigma>'\<rparr> |:| R)"
+                                and t="LIf t1 t2 t3", 
                                 simplified "subterm_set.distinct" HOL.simp_thms , rule_format, OF has_type_LIf(9), simplified,
-                                rule_format,split_and_rule]
+                                split_and_rule]
             ) 
       using has_type_LIf(2,4,6,7,8)
       apply (fastforce intro!: has_type_L.intros)+
       done
 next
-  case (has_type_LAbs \<Gamma>1 T1 t2 \<delta>1 T2)
-    have 1:"\<And>p R n. p \<in> set (patterns t2) \<Longrightarrow> \<Gamma>' \<turnstile> \<lparr><|V p|>|;|fill \<delta>\<rparr> |:| R \<Longrightarrow> insert_nth n S \<Gamma>' \<turnstile> \<lparr><|V p|>|;|fill \<delta>'\<rparr> |:| R"
-      using has_type_LAbs(5) subterms.simps 
-            P_set_Pat[where P="\<lambda>x. (\<forall> R n . \<Gamma>' \<turnstile> \<lparr><|V x|>|;|fill \<delta>\<rparr> |:| R \<longrightarrow> insert_nth n S \<Gamma>' \<turnstile> \<lparr><|V x|>|;|fill \<delta>'\<rparr> |:| R)" and
-                            t = "LAbs T1 t2"]
+  case (has_type_LAbs \<Gamma>1 T1 t2 \<sigma>1 T2)
+    have 1:"\<And>p R n. p \<in> set (patterns t2) \<Longrightarrow> \<Gamma>' \<turnstile> \<lparr><|V p|>|;|fill \<sigma>\<rparr> |:| R \<Longrightarrow> insert_nth n S \<Gamma>' \<turnstile> \<lparr><|V p|>|;|fill \<sigma>'\<rparr> |:| R"
+      using P_pat_subterm_cases[where P="\<lambda>pt. (\<forall> x R n . x\<in>set pt \<longrightarrow> \<Gamma>' \<turnstile> \<lparr><|V x|>|;|fill \<sigma>\<rparr> |:| R \<longrightarrow> insert_nth n S \<Gamma>' \<turnstile> \<lparr><|V x|>|;|fill \<sigma>'\<rparr> |:| R)" and
+                                  t = "LAbs T1 t2", simplified "subterm_set.distinct" HOL.simp_thms , rule_format,
+                                  OF has_type_LAbs(5)]
       by force
+
     have 2:"Suc n\<le>length(\<Gamma>1|,|T1)" using has_type_LAbs(4) by auto
-    have "insert_nth (Suc n) S (\<Gamma>1 |,| T1) \<turnstile> \<lparr>shift_L 1 (Suc n) t2|;|fill \<delta>'\<rparr> |:| T2"
-      using has_type_LAbs(2)[OF has_type_LAbs(3) 2, of \<Gamma>' \<delta>'] 1 
+
+    have "insert_nth (Suc n) S (\<Gamma>1 |,| T1) \<turnstile> \<lparr>shift_L 1 (Suc n) t2|;|fill \<sigma>'\<rparr> |:| T2"
+      using has_type_LAbs(2)[OF has_type_LAbs(3) 2, of \<Gamma>' \<sigma>'] 1 
       by fast
     then show ?case
-      using "has_type_L.intros"(9)[of T1 "insert_nth n S \<Gamma>1" "shift_L 1 n t2" \<delta> T2]
+      using "has_type_L.intros"(9)[of T1 "insert_nth n S \<Gamma>1" "shift_L 1 n t2" \<sigma> T2]
             has_type_L.has_type_LAbs 
       by auto              
 next 
-  case(has_type_Tuple L TL \<Gamma>1 \<delta>1)
-    have 1:"\<And>i. i<length L \<Longrightarrow> (\<And>p R n. p \<in> set (patterns (L ! i)) \<Longrightarrow> \<Gamma>' \<turnstile> \<lparr><|V p|>|;|fill \<delta>\<rparr> |:| R \<Longrightarrow> 
-                    insert_nth n S \<Gamma>' \<turnstile> \<lparr><|V p|>|;|fill \<delta>'\<rparr> |:| R)"
+  case(has_type_Tuple L TL \<Gamma>1 \<sigma>1)
+    have 1:"\<And>i. i<length L \<Longrightarrow> (\<And>p R n. p \<in> set (patterns (L ! i)) \<Longrightarrow> \<Gamma>' \<turnstile> \<lparr><|V p|>|;|fill \<sigma>\<rparr> |:| R \<Longrightarrow> 
+                    insert_nth n S \<Gamma>' \<turnstile> \<lparr><|V p|>|;|fill \<sigma>'\<rparr> |:| R)"
       using has_type_Tuple(7)[unfolded patterns.simps(12) set_list_it_app set_map]
             set_conv_nth[of L]
       by blast      
     show ?case    
       using has_type_Tuple(1,2) nth_map[of _ L "shift_L 1 n"] 1
-            has_type_Tuple(4)[OF _ _ has_type_Tuple(5,6), of _ \<Gamma>' \<delta>']
+            has_type_Tuple(4)[OF _ _ has_type_Tuple(5,6), of _ \<Gamma>' \<sigma>']
       by (force intro!: has_type_L.intros(18))+
 next
-  case (has_type_ProjT i TL \<Gamma>1 t \<delta>1)
+  case (has_type_ProjT i TL \<Gamma>1 t \<sigma>1)
     show ?case
-      using has_type_ProjT(4)[OF has_type_ProjT(5,6),of \<Gamma>' \<delta>']
+      using has_type_ProjT(4)[OF has_type_ProjT(5,6),of \<Gamma>' \<sigma>']
             "has_type_L.intros"(19)[OF has_type_ProjT(1,2)]
             has_type_ProjT(7)
       by fastforce
 next
-  case (has_type_RCD L LT TL \<Gamma> \<delta>1)
+  case (has_type_RCD L LT TL \<Gamma> \<sigma>1)
     have " \<And>i. i < length LT \<Longrightarrow> (\<And>p R n. p \<in> set (patterns (LT ! i)) \<Longrightarrow> 
-            \<Gamma>' \<turnstile> \<lparr><|V p|>|;|fill \<delta>\<rparr> |:| R \<Longrightarrow> insert_nth n S \<Gamma>' \<turnstile> \<lparr><|V p|>|;|fill \<delta>'\<rparr> |:| R)"
+            \<Gamma>' \<turnstile> \<lparr><|V p|>|;|fill \<sigma>\<rparr> |:| R \<Longrightarrow> insert_nth n S \<Gamma>' \<turnstile> \<lparr><|V p|>|;|fill \<sigma>'\<rparr> |:| R)"
       using set_conv_nth[of LT]
             has_type_RCD(9)[unfolded patterns.simps(13) set_list_it_app set_map]
       by blast
@@ -476,146 +466,144 @@ next
             has_type_RCD(6)[OF _ has_type_RCD(7,8)]           
       by (force intro!: "has_type_L.intros"(20))+
 next
-  case (has_type_Let \<Gamma>1 t1 \<delta>1 A x t2 B)
-    have H:"\<And>p R n. p \<in> set (patterns t1) \<Longrightarrow> \<Gamma>' \<turnstile> \<lparr><|V p|>|;|fill \<delta>\<rparr> |:| R \<Longrightarrow> insert_nth n S \<Gamma>' \<turnstile> \<lparr><|V p|>|;|fill \<delta>'\<rparr> |:| R"
-       "\<And>p R n. p \<in> set (patterns t2) \<Longrightarrow> \<Gamma>' \<turnstile> \<lparr><|V p|>|;|fill \<delta>\<rparr> |:| R \<Longrightarrow> insert_nth n S \<Gamma>' \<turnstile> \<lparr><|V p|>|;|fill \<delta>'\<rparr> |:| R"
+  case (has_type_Let \<Gamma> t1 \<sigma>1 A x t2 B)
+    have H:"\<And>p R n. p \<in> set (patterns t1) \<Longrightarrow> \<Gamma>' \<turnstile> \<lparr><|V p|>|;|fill \<sigma>\<rparr> |:| R \<Longrightarrow> insert_nth n S \<Gamma>' \<turnstile> \<lparr><|V p|>|;|fill \<sigma>'\<rparr> |:| R"
+       "\<And>p R n. p \<in> set (patterns t2) \<Longrightarrow> \<Gamma>' \<turnstile> \<lparr><|V p|>|;|fill \<sigma>\<rparr> |:| R \<Longrightarrow> insert_nth n S \<Gamma>' \<turnstile> \<lparr><|V p|>|;|fill \<sigma>'\<rparr> |:| R"
       using has_type_Let(7)[unfolded patterns.simps(10) set_append]
       by blast+
-
-    have 1:"n\<le>x \<Longrightarrow> ?case"
-      proof -
-        assume le_x: "n\<le>x"
-        from H show ?case
-          using has_type_Let(6) has_type_Let(4)[OF has_type_Let(5), of n \<Gamma>' \<delta>'] le_x
-                "has_type_L.intros"(14)[OF has_type_Let(2)[OF has_type_Let(5,6)], of \<Gamma>' \<delta>' "Suc x"]
-          by (simp add: le_x del: Fun.comp_apply insert_nth_take_drop, 
-                metis rep_ins replace_inv_length)
-      qed
-
-    from H have "n>x \<Longrightarrow> ?case"
-      using has_type_Let(4-6) rep_ins2[OF _ has_type_Let(6), of x S A]
-            "has_type_L.intros"(14)[OF has_type_Let(2)[OF has_type_Let(5,6)], of \<Gamma>' \<delta>' x]
-      by (simp del: Fun.comp_apply insert_nth_take_drop,
-            metis replace_inv_length)
-    with 1 show ?case 
-      by auto
+    have "n \<le> x \<Longrightarrow> (take n \<Gamma> @ drop n \<Gamma> |,| S) \<turnstile> \<lparr>Let var Suc x := shift_L 1 n t1 in shift_L 1 n t2|;|fill \<sigma>'\<rparr> |:| B"
+      using has_type_Let(2)[OF has_type_Let(5,6)] H(1)
+            has_type_Let(4)[unfolded length_insert_nth, OF has_type_Let(5), of n \<Gamma>' \<sigma>'] H(2) has_type_Let(6)
+            insert_nth_comp(1)[OF has_type_Let(6), of x S A] 
+      by (auto intro!: has_type_L.intros(14))  
+    then show ?case
+      using has_type_Let(2)[OF has_type_Let(5,6)] H(1)
+            has_type_Let(4)[unfolded length_insert_nth, OF has_type_Let(5), of "Suc n" \<Gamma>' \<sigma>'] H(2) has_type_Let(6)
+            insert_nth_comp(2)[OF has_type_Let(6),of x S A]  
+      by (auto intro!: has_type_L.intros(14)) 
 next
-  case (has_type_PatternVar \<Gamma>1 \<delta>1 m k A)
-    have 1:"insert_nth n S \<Gamma>1 \<turnstile> \<lparr>(fill \<delta>' ^^ m) (<|V k|>)|;|id\<rparr> |:| A" 
-      using has_type_PatternVar(2)[of _ \<Gamma>' "\<lambda>x. <|V x|>",
-                                    unfolded has_type_PatternVar(3,4)]
-            fill_id[symmetric]
-            has_type_PatternVar(6)[of k]
-      apply (simp del: insert_nth_take_drop)      
+  case (has_type_PatternVar \<Gamma>1 \<sigma>1 m k A)
+    note hyps=this
+    show ?case
+      apply simp
+      apply rule
+      using hyps(2)[OF hyps(4,5), unfolded hyps(3), simplified]
+            hyps(3,6) 
       sorry
-    have "set (patterns ((fill \<delta>' ^^ m) (<|V k|>))) = {}"
-      using has_type_PatternVar(3,4) pattern_fill_shift[of m 1 n \<delta> "<|V k|>"]
-      sorry  
-    with 1 show ?case 
-      by (auto intro:"has_type_L.intros"(22))
 next
-  case (has_type_LetPattern p t1 \<delta>1 \<Gamma>1 \<delta>2 B t2 A n \<delta>3 \<Gamma>')
-    have H: "\<And>p' R n. p' \<in> set (patterns t1) \<Longrightarrow> \<Gamma>' \<turnstile> \<lparr><|V p'|>|;|fill \<delta>\<rparr> |:| R \<Longrightarrow> 
-                  insert_nth n S \<Gamma>' \<turnstile> \<lparr><|V p'|>|;|fill \<delta>3\<rparr> |:| R"
-            "\<And>p' R n. p' \<in>  {x \<in> set (patterns t2). x \<notin> set (Pvars p)} \<Longrightarrow> 
-              \<Gamma>' \<turnstile> \<lparr><|V p'|>|;|fill \<delta>\<rparr> |:| R \<Longrightarrow> insert_nth n S \<Gamma>' \<turnstile> \<lparr><|V p'|>|;|fill \<delta>3\<rparr> |:| R"
-      using has_type_LetPattern(9)[unfolded patterns.simps set_append set_filter]
+  case (has_type_LetPattern p t1 \<sigma>1 \<Gamma> t2 \<sigma>2 A \<sigma>t n \<sigma>3 \<Gamma>')
+    note hyps=this
+    have H: "\<And>p' R n. p' \<in> set (patterns t1) \<Longrightarrow> \<Gamma>' \<turnstile> \<lparr><|V p'|>|;|fill \<sigma>t\<rparr> |:| R \<Longrightarrow> 
+                  insert_nth n S \<Gamma>' \<turnstile> \<lparr><|V p'|>|;|fill \<sigma>3\<rparr> |:| R"
+            "\<And>p' R n. p' \<in> set (patterns t2) \<Longrightarrow> 
+              \<Gamma>' \<turnstile> \<lparr><|V p'|>|;|fill \<sigma>t\<rparr> |:| R \<Longrightarrow> insert_nth n S \<Gamma>' \<turnstile> \<lparr><|V p'|>|;|fill \<sigma>3\<rparr> |:| R"
+      using P_pat_subterm_cases[where P="\<lambda>pt. (\<forall> x R n. x\<in>set pt \<longrightarrow> \<Gamma>' \<turnstile> \<lparr><|V x|>|;|fill \<sigma>t\<rparr> |:| R \<longrightarrow> insert_nth n S \<Gamma>' \<turnstile> \<lparr><|V x|>|;|fill \<sigma>3\<rparr> |:| R)"
+                                and t="Let pattern p := t1 in t2",
+                                simplified subterms.simps "subterm_set.distinct" HOL.simp_thms,
+                                rule_format] hyps(7)
       by blast+
-    have 1:"Lmatch p (shift_L 1 n t1) (shift_L 1 n \<circ> \<delta>1)"
+    have 1:"Lmatch p (shift_L 1 n t1) (shift_L 1 n \<circ> \<sigma>1)"
       sorry
-    obtain \<delta>' where fill_\<delta>1:"\<delta>1 = fill \<delta>'"
+    obtain \<sigma>' where fill_\<sigma>1:"\<sigma>1 = fill \<sigma>'"
       using lmatch_gives_fill[OF has_type_LetPattern(2)]
       by auto
-    hence "insert_nth n S \<Gamma>1 \<turnstile> \<lparr>shift_L 1 n t2|;|(fill \<delta>3 \<circ> (shift_L 1 n \<circ> \<delta>1))\<rparr> |:| A"
-      using H(2)
+    obtain \<sigma>4 where shifted_fill:"(shift_L 1 n \<circ> \<sigma>1) = fill \<sigma>4"
+      using lmatch_gives_fill[OF 1]
+      by metis
+    have 2: " (\<And>p R n. p \<in> set (patterns t2) \<Longrightarrow>
+              \<Gamma>' \<turnstile> \<lparr><|V p|>|;|fill (fill \<sigma>2 \<circ> \<sigma>')\<rparr> |:| R \<Longrightarrow>
+              insert_nth n S \<Gamma>' \<turnstile> \<lparr><|V p|>|;|fill (fill \<sigma>3 \<circ> \<sigma>4)\<rparr> |:| R)"
+      nitpick
       sorry
-    then show ?case
-      using has_type_LetPattern(1)
-            1 has_type_LetPattern(4)[OF has_type_LetPattern(7,8), of \<Gamma>' \<delta>3]
-            H(1)
+    show ?case
+      using has_type_LetPattern(1) 1
+            has_type_LetPattern(4)[of "fill \<sigma>2 \<circ> \<sigma>'" n \<Gamma>' "fill \<sigma>3 \<circ> \<sigma>4", 
+                                   OF _ has_type_LetPattern(6)] 
+            H(2)[unfolded has_type_LetPattern(5)[symmetric]] fill_\<sigma>1
+            shifted_fill fill_fill_comp 2
       by (auto intro: has_type_L.intros(24))
 next
-  case (has_type_Case \<Gamma>1 t \<delta>1 A B x t1 C y t2)
-    have H:"\<And>p R n. p \<in> set (patterns t) \<Longrightarrow> \<Gamma>' \<turnstile> \<lparr><|V p|>|;|fill \<delta>\<rparr> |:| R \<Longrightarrow> insert_nth n S \<Gamma>' \<turnstile> \<lparr><|V p|>|;|fill \<delta>'\<rparr> |:| R"
-           "\<And>p R n. p \<in> set (patterns t1) \<Longrightarrow> \<Gamma>' \<turnstile> \<lparr><|V p|>|;|fill \<delta>\<rparr> |:| R \<Longrightarrow> insert_nth n S \<Gamma>' \<turnstile> \<lparr><|V p|>|;|fill \<delta>'\<rparr> |:| R"
-           "\<And>p R n. p \<in> set (patterns t2) \<Longrightarrow> \<Gamma>' \<turnstile> \<lparr><|V p|>|;|fill \<delta>\<rparr> |:| R \<Longrightarrow> insert_nth n S \<Gamma>' \<turnstile> \<lparr><|V p|>|;|fill \<delta>'\<rparr> |:| R"
+  case (has_type_Case \<Gamma>1 t \<sigma>1 A B x t1 C y t2)
+    have H:"\<And>p R n. p \<in> set (patterns t) \<Longrightarrow> \<Gamma>' \<turnstile> \<lparr><|V p|>|;|fill \<sigma>\<rparr> |:| R \<Longrightarrow> insert_nth n S \<Gamma>' \<turnstile> \<lparr><|V p|>|;|fill \<sigma>'\<rparr> |:| R"
+           "\<And>p R n. p \<in> set (patterns t1) \<Longrightarrow> \<Gamma>' \<turnstile> \<lparr><|V p|>|;|fill \<sigma>\<rparr> |:| R \<Longrightarrow> insert_nth n S \<Gamma>' \<turnstile> \<lparr><|V p|>|;|fill \<sigma>'\<rparr> |:| R"
+           "\<And>p R n. p \<in> set (patterns t2) \<Longrightarrow> \<Gamma>' \<turnstile> \<lparr><|V p|>|;|fill \<sigma>\<rparr> |:| R \<Longrightarrow> insert_nth n S \<Gamma>' \<turnstile> \<lparr><|V p|>|;|fill \<sigma>'\<rparr> |:| R"
       using has_type_Case(9)[unfolded patterns.simps set_append]
       by blast+
-    have A: "insert_nth n S \<Gamma>1 \<turnstile> \<lparr>shift_L 1 n t|;|fill \<delta>'\<rparr> |:| A |+| B"
+    have A: "insert_nth n S \<Gamma>1 \<turnstile> \<lparr>shift_L 1 n t|;|fill \<sigma>'\<rparr> |:| A |+| B"
       using has_type_Case(2)[OF has_type_Case(7,8)] H(1)
       by auto
-    have B1:"n \<le> x \<Longrightarrow> n \<le> y \<Longrightarrow> replace (Suc x) A (insert_nth n S \<Gamma>1) \<turnstile> \<lparr>shift_L 1 n t1|;|fill \<delta>'\<rparr> |:| C \<and>
-                                  replace (Suc y) B (insert_nth n S \<Gamma>1) \<turnstile> \<lparr>shift_L 1 n t2|;|fill \<delta>'\<rparr> |:| C"
-      using  has_type_Case(4)[OF has_type_Case(7)] has_type_Case(8)
-             has_type_Case(6)[OF has_type_Case(7)] H(2,3)
-             rep_ins[of n _ \<Gamma>1 S _] replace_inv_length 
-      by metis+
-    have B2: " n \<le> x \<Longrightarrow> \<not> n \<le> y \<Longrightarrow> replace (Suc x) A (insert_nth n S \<Gamma>1) \<turnstile> \<lparr>shift_L 1 n t1|;|fill \<delta>'\<rparr> |:| C \<and>
-                                      replace y B (insert_nth n S \<Gamma>1) \<turnstile> \<lparr>shift_L 1 n t2|;|fill \<delta>'\<rparr> |:| C"
-      using  has_type_Case(4)[OF has_type_Case(7)] has_type_Case(8) H(2,3)
-             has_type_Case(6)[OF has_type_Case(7)] rep_ins2[of y n \<Gamma>1 S B]
-             rep_ins[of n x \<Gamma>1 S A] replace_inv_length not_le
-      by metis+
-    have B3: "\<not> n \<le> x \<Longrightarrow>  n \<le> y \<Longrightarrow> replace x A (insert_nth n S \<Gamma>1) \<turnstile> \<lparr>shift_L 1 n t1|;|fill \<delta>'\<rparr> |:| C \<and>
-                                      replace (Suc y) B (insert_nth n S \<Gamma>1) \<turnstile> \<lparr>shift_L 1 n t2|;|fill \<delta>'\<rparr> |:| C"
+    have B1:"n \<le> x \<Longrightarrow> n \<le> y \<Longrightarrow> insert_nth (Suc x) A (insert_nth n S \<Gamma>1) \<turnstile> \<lparr>shift_L 1 n t1|;|fill \<sigma>'\<rparr> |:| C \<and>
+                                  insert_nth (Suc y) B (insert_nth n S \<Gamma>1) \<turnstile> \<lparr>shift_L 1 n t2|;|fill \<sigma>'\<rparr> |:| C"
+      using  has_type_Case(4)[OF has_type_Case(7),of n \<Gamma>' \<sigma>'] has_type_Case(8)
+             has_type_Case(6)[OF has_type_Case(7),of n \<Gamma>' \<sigma>'] H(2,3)
+             insert_nth_comp(1)[of n \<Gamma>1 _ S _] length_insert_nth
+      by (metis le_SucI)+
+    have B2: " n \<le> x \<Longrightarrow> \<not> n \<le> y \<Longrightarrow>  insert_nth (Suc x) A (insert_nth n S \<Gamma>1) \<turnstile> \<lparr>shift_L 1 n t1|;|fill \<sigma>'\<rparr> |:| C \<and>
+                                      insert_nth y B (insert_nth n S \<Gamma>1) \<turnstile> \<lparr>shift_L 1 n t2|;|fill \<sigma>'\<rparr> |:| C"
+      using  has_type_Case(4)[OF has_type_Case(7)]
+             has_type_Case(6)[OF has_type_Case(7)]  has_type_Case(8) H(2,3)
+             insert_nth_comp(2)[of n _ y S B, symmetric] length_insert_nth not_le
+      sorry
+    have B3: "\<not> n \<le> x \<Longrightarrow>  n \<le> y \<Longrightarrow> insert_nth x A (insert_nth n S \<Gamma>1) \<turnstile> \<lparr>shift_L 1 n t1|;|fill \<sigma>'\<rparr> |:| C \<and>
+                                      insert_nth (Suc y) B (insert_nth n S \<Gamma>1) \<turnstile> \<lparr>shift_L 1 n t2|;|fill \<sigma>'\<rparr> |:| C"
       using  has_type_Case(4)[OF has_type_Case(7)] has_type_Case(8) H(2,3)
              has_type_Case(6)[OF has_type_Case(7)] rep_ins2[of x n \<Gamma>1 S A]
              rep_ins[of n y \<Gamma>1 S B] replace_inv_length not_le
-      by metis+
-    have B4: "\<not> n \<le> x \<Longrightarrow> \<not> n \<le> y \<Longrightarrow> replace x A (insert_nth n S \<Gamma>1) \<turnstile> \<lparr>shift_L 1 n t1|;|fill \<delta>'\<rparr> |:| C \<and>
-                                      replace y B (insert_nth n S \<Gamma>1) \<turnstile> \<lparr>shift_L 1 n t2|;|fill \<delta>'\<rparr> |:| C"
+      sorry
+    have B4: "\<not> n \<le> x \<Longrightarrow> \<not> n \<le> y \<Longrightarrow> insert_nth x A (insert_nth n S \<Gamma>1) \<turnstile> \<lparr>shift_L 1 n t1|;|fill \<sigma>'\<rparr> |:| C \<and>
+                                      insert_nth y B (insert_nth n S \<Gamma>1) \<turnstile> \<lparr>shift_L 1 n t2|;|fill \<sigma>'\<rparr> |:| C"
       using  has_type_Case(4)[OF has_type_Case(7)] has_type_Case(8) H(2,3)
-             has_type_Case(6)[OF has_type_Case(7)] rep_ins2[of _ n \<Gamma>1 S _]
-             replace_inv_length not_le
-      by metis+
+             has_type_Case(6)[OF has_type_Case(7)]
+             insert_nth_comp not_le
+      sorry
     show ?case
       by (auto)(insert A B1 B2 B3 B4 "has_type_L.intros"(27), force+)
 next
-  case (has_type_CaseV L I TL LT \<Gamma> t \<delta>1 A)
-    have filledH: "\<And>p R n. p \<in> set (patterns t) \<Longrightarrow> \<Gamma>' \<turnstile> \<lparr><|V p|>|;|fill \<delta>\<rparr> |:| R \<Longrightarrow> insert_nth n S \<Gamma>' \<turnstile> \<lparr><|V p|>|;|fill \<delta>'\<rparr> |:| R"
-            "\<And>i. i<length LT \<Longrightarrow> (\<And>p R n. p \<in> set (patterns (LT!i)) \<Longrightarrow> \<Gamma>' \<turnstile> \<lparr><|V p|>|;|fill \<delta>\<rparr> |:| R \<Longrightarrow> insert_nth n S \<Gamma>' \<turnstile> \<lparr><|V p|>|;|fill \<delta>'\<rparr> |:| R)"
+  case (has_type_CaseV L I TL LT \<Gamma> t \<sigma>1 A)
+    have filledH: "\<And>p R n. p \<in> set (patterns t) \<Longrightarrow> \<Gamma>' \<turnstile> \<lparr><|V p|>|;|fill \<sigma>\<rparr> |:| R \<Longrightarrow> insert_nth n S \<Gamma>' \<turnstile> \<lparr><|V p|>|;|fill \<sigma>'\<rparr> |:| R"
+            "\<And>i. i<length LT \<Longrightarrow> (\<And>p R n. p \<in> set (patterns (LT!i)) \<Longrightarrow> \<Gamma>' \<turnstile> \<lparr><|V p|>|;|fill \<sigma>\<rparr> |:| R \<Longrightarrow> insert_nth n S \<Gamma>' \<turnstile> \<lparr><|V p|>|;|fill \<sigma>'\<rparr> |:| R)"
       using has_type_CaseV(10)[unfolded patterns.simps set_append set_list_it_app set_map]
             set_conv_nth[of LT]
       by blast+
     have branches_wtyped:"\<forall>i<length L.
        replace (map (\<lambda>x. if n \<le> x then nat (int x + 1) else x) I ! i) (TL ! i) (take n \<Gamma> @ drop n \<Gamma> |,| S)
-       \<turnstile> \<lparr>(map (shift_L 1 n) LT ! i)|;|fill \<delta>'\<rparr> |:| A"
+       \<turnstile> \<lparr>(map (shift_L 1 n) LT ! i)|;|fill \<sigma>'\<rparr> |:| A"
       proof (rule+)
         fix i
         assume H:"i<length L"
         have "\<And>x. x\<le>length (replace (I ! i) (TL ! i) \<Gamma>) \<Longrightarrow>
             \<forall>xa xb. (\<forall>x. x \<in> set (patterns (LT ! i)) \<longrightarrow>
-                         (\<forall>xc. xb \<turnstile> \<lparr><|V x|>|;|fill \<delta>\<rparr> |:| xc \<longrightarrow> (\<forall>xd. insert_nth xd S xb \<turnstile> \<lparr><|V x|>|;|fill xa\<rparr> |:| xc))) \<longrightarrow>
+                         (\<forall>xc. xb \<turnstile> \<lparr><|V x|>|;|fill \<sigma>\<rparr> |:| xc \<longrightarrow> (\<forall>xd. insert_nth xd S xb \<turnstile> \<lparr><|V x|>|;|fill xa\<rparr> |:| xc))) \<longrightarrow>
                     insert_nth x S (replace (I ! i) (TL ! i) \<Gamma>) \<turnstile> \<lparr>shift_L 1 x (LT ! i)|;|fill xa\<rparr> |:| A"
           using has_type_CaseV(7,8) H 
           by auto
-        then have branches_type:"insert_nth n S (replace (I ! i) (TL ! i) \<Gamma>) \<turnstile> \<lparr>shift_L 1 n (LT ! i)|;|fill \<delta>'\<rparr> |:| A"
+        then have branches_type:"insert_nth n S (replace (I ! i) (TL ! i) \<Gamma>) \<turnstile> \<lparr>shift_L 1 n (LT ! i)|;|fill \<sigma>'\<rparr> |:| A"
           using  has_type_CaseV(9) filledH(2)[OF H[unfolded has_type_CaseV(4)]]   
                  replace_inv_length[of "I!i" "TL!i" \<Gamma>]
           by metis
         have 1:"n\<le> I!i \<Longrightarrow> replace (map (\<lambda>x. if n \<le> x then nat (int x + 1) else x) I ! i) (TL ! i) (take n \<Gamma> @ drop n \<Gamma> |,| S)
-                \<turnstile> \<lparr>(map (shift_L 1 n) LT ! i)|;|fill \<delta>'\<rparr> |:| A"
+                \<turnstile> \<lparr>(map (shift_L 1 n) LT ! i)|;|fill \<sigma>'\<rparr> |:| A"
           using has_type_CaseV(1,2,9) H        
           proof -
             
             assume hyps:"n \<le> I ! i" "L \<noteq> \<emptyset>" "length I = length L" "n \<le> length \<Gamma>" "i < length L"
             
             from branches_type
-              have "replace (Suc (I ! i)) (TL ! i) (take n \<Gamma> @ drop n \<Gamma> |,| S) \<turnstile> \<lparr>(map (shift_L 1 n) LT ! i)|;|fill \<delta>'\<rparr> |:| A"
+              have "replace (Suc (I ! i)) (TL ! i) (take n \<Gamma> @ drop n \<Gamma> |,| S) \<turnstile> \<lparr>(map (shift_L 1 n) LT ! i)|;|fill \<sigma>'\<rparr> |:| A"
               using rep_ins[OF hyps(1,4),of S "TL!i"] H has_type_CaseV(4)
               by auto
             
             then show ?thesis by (simp add: hyps)        
           qed
         have  "\<not> n\<le> I!i \<Longrightarrow> replace (map (\<lambda>x. if n \<le> x then nat (int x + 1) else x) I ! i) (TL ! i) (take n \<Gamma> @ drop n \<Gamma> |,| S)
-                \<turnstile> \<lparr>(map (shift_L 1 n) LT ! i)|;|fill \<delta>'\<rparr> |:| A"
+                \<turnstile> \<lparr>(map (shift_L 1 n) LT ! i)|;|fill \<sigma>'\<rparr> |:| A"
           using has_type_CaseV(1,2,9) H        
           proof -
             
             assume hyps:"\<not>n \<le> I ! i" "L \<noteq> \<emptyset>" "length I = length L" "n \<le> length \<Gamma>" "i < length L"
             
             from branches_type
-              have  "replace (I ! i) (TL ! i) (take n \<Gamma> @ drop n \<Gamma> |,| S) \<turnstile> \<lparr>(map (shift_L 1 n) LT ! i)|;|fill \<delta>'\<rparr> |:| A"
+              have  "replace (I ! i) (TL ! i) (take n \<Gamma> @ drop n \<Gamma> |,| S) \<turnstile> \<lparr>(map (shift_L 1 n) LT ! i)|;|fill \<sigma>'\<rparr> |:| A"
               using rep_ins2[OF _ hyps(4),of "I!i" S "TL!i"] H has_type_CaseV(4) hyps(1) not_le[of n "I!i"]
               by auto
 
@@ -623,7 +611,7 @@ next
           qed
 
         with 1 show "replace (map (\<lambda>x. if n \<le> x then nat (int x + 1) else x) I ! i) (TL ! i) (take n \<Gamma> @ drop n \<Gamma> |,| S)
-         \<turnstile> \<lparr>(map (shift_L 1 n) LT ! i)|;|fill \<delta>'\<rparr> |:| A"
+         \<turnstile> \<lparr>(map (shift_L 1 n) LT ! i)|;|fill \<sigma>'\<rparr> |:| A"
           by blast
       qed 
     show ?case
@@ -633,21 +621,21 @@ next
 qed (auto intro!: has_type_L.intros simp: nth_append min_def)
 
 lemma fill_keep_value:
-  "is_value_L v \<Longrightarrow> is_value_L (fill \<delta> v)"
+  "is_value_L v \<Longrightarrow> is_value_L (fill \<sigma> v)"
 by(induction v rule: is_value_L.induct, auto intro: "is_value_L.intros" )
 
 lemma canonical_forms:
-  "is_value_L v \<Longrightarrow> \<Gamma> \<turnstile> \<lparr>v|;|\<delta>\<rparr> |:| Bool \<Longrightarrow> v = LTrue \<or> v = LFalse"
-  "is_value_L v \<Longrightarrow> \<Gamma> \<turnstile> \<lparr>v|;|\<delta>\<rparr> |:| T1 \<rightarrow> T2 \<Longrightarrow> \<exists>t n. v = LAbs T1 t"
-  "is_value_L v \<Longrightarrow> \<Gamma> \<turnstile> \<lparr>v|;|\<delta>\<rparr> |:| Unit \<Longrightarrow> v = unit"
-  "is_value_L v \<Longrightarrow> \<Gamma> \<turnstile> \<lparr>v|;|\<delta>\<rparr> |:| A |\<times>| B \<Longrightarrow> \<exists>v1 v2. is_value_L v1 \<and> is_value_L v2 \<and> v= \<lbrace>v1,v2\<rbrace>"
-  "is_value_L v \<Longrightarrow> \<Gamma> \<turnstile> \<lparr>v|;|\<delta>\<rparr> |:| \<lparr>TL\<rparr> \<Longrightarrow> \<exists>L. is_value_L (Tuple L) \<and> v = Tuple L"
-  "is_value_L v \<Longrightarrow> \<Gamma> \<turnstile> \<lparr>v|;|\<delta>\<rparr> |:| \<lparr>L|:|TL\<rparr> \<Longrightarrow> \<exists>L LT. is_value_L (Record L LT) \<and> v = (Record L LT)" 
-  "is_value_L v \<Longrightarrow> \<Gamma> \<turnstile> \<lparr>v|;|\<delta>\<rparr> |:| A|+|B \<Longrightarrow> (\<exists>v1. is_value_L v1 \<and> v = inl v1 as A|+|B) \<or> (\<exists>v1. v = inr v1 as A|+|B \<and> is_value_L v1)" 
-  "is_value_L v \<Longrightarrow> \<Gamma> \<turnstile> \<lparr>v|;|\<delta>\<rparr> |:| Nat \<Longrightarrow> \<exists>n. v = LNat n"
+  "is_value_L v \<Longrightarrow> \<Gamma> \<turnstile> \<lparr>v|;|\<sigma>\<rparr> |:| Bool \<Longrightarrow> v = LTrue \<or> v = LFalse"
+  "is_value_L v \<Longrightarrow> \<Gamma> \<turnstile> \<lparr>v|;|\<sigma>\<rparr> |:| T1 \<rightarrow> T2 \<Longrightarrow> \<exists>t n. v = LAbs T1 t"
+  "is_value_L v \<Longrightarrow> \<Gamma> \<turnstile> \<lparr>v|;|\<sigma>\<rparr> |:| Unit \<Longrightarrow> v = unit"
+  "is_value_L v \<Longrightarrow> \<Gamma> \<turnstile> \<lparr>v|;|\<sigma>\<rparr> |:| A |\<times>| B \<Longrightarrow> \<exists>v1 v2. is_value_L v1 \<and> is_value_L v2 \<and> v= \<lbrace>v1,v2\<rbrace>"
+  "is_value_L v \<Longrightarrow> \<Gamma> \<turnstile> \<lparr>v|;|\<sigma>\<rparr> |:| \<lparr>TL\<rparr> \<Longrightarrow> \<exists>L. is_value_L (Tuple L) \<and> v = Tuple L"
+  "is_value_L v \<Longrightarrow> \<Gamma> \<turnstile> \<lparr>v|;|\<sigma>\<rparr> |:| \<lparr>L|:|TL\<rparr> \<Longrightarrow> \<exists>L LT. is_value_L (Record L LT) \<and> v = (Record L LT)" 
+  "is_value_L v \<Longrightarrow> \<Gamma> \<turnstile> \<lparr>v|;|\<sigma>\<rparr> |:| A|+|B \<Longrightarrow> (\<exists>v1. is_value_L v1 \<and> v = inl v1 as A|+|B) \<or> (\<exists>v1. v = inr v1 as A|+|B \<and> is_value_L v1)" 
+  "is_value_L v \<Longrightarrow> \<Gamma> \<turnstile> \<lparr>v|;|\<sigma>\<rparr> |:| Nat \<Longrightarrow> \<exists>n. v = LNat n"
 proof -
   assume  val: "is_value_L v" and 
-          typed: "\<Gamma> \<turnstile> \<lparr>v|;|\<delta>\<rparr> |:| A|+|B"
+          typed: "\<Gamma> \<turnstile> \<lparr>v|;|\<sigma>\<rparr> |:| A|+|B"
   show "(\<exists>v1. is_value_L v1 \<and> v = inl v1 as A|+|B) \<or> (\<exists>v1. v = inr v1 as A|+|B \<and> is_value_L v1)"
     using val typed
     by (induction rule: is_value_L.induct, auto elim: "has_type_L.cases")
